hol/table_arith_to_intervalScript.sml
@@ -1,0 +1,1393 @@
+open HolKernel boolLib liteLib simpLib Parse bossLib;
+open arithmeticTheory stringTheory containerTheory pred_setTheory
+     listTheory finite_mapTheory;
+
+open p4Lib;
+open blastLib bitstringLib;
+open p4Theory;
+open p4_auxTheory;
+open p4_coreTheory;
+
+open bitstringTheory;
+open wordsTheory;
+open optionTheory;
+open sumTheory;
+open stringTheory;
+open ottTheory;
+open pairTheory;
+open rich_listTheory;
+open arithmeticTheory;
+open alistTheory;
+open numeralTheory;
+open alistTheory;
+open set_relationTheory;
+open pred_setTheory;
+open pred_setLib;
+
+open bdd_genTheory;     
+open pred_specTheory;     
+open policy_specTheory;     
+open tables_specTheory;
+
+open table_bs_propertiesTheory;
+     
+open policy_arith_to_varTheory;
+open table_var_to_arithTheory;
+
+val _ = new_theory "table_arith_to_interval";
+
+
+(*==========================================*)
+(*         Types of interval tables         *)
+(*==========================================*)       
+val _ = Hol_datatype ` 
+  interval = Empty | Single of bitv => bitv
+`;
+
+val _ = Hol_datatype ` 
+  interval_key = key_val of arith_lv | key_const of bitv
+`;
+
+        
+Type intvl_row        = “:(interval list # num # 'a action_expr)”;
+Type intvl_table      = “:(interval_key # 'a intvl_row list)”;
+Type intvl_table_list = “:('a intvl_table ) list”;
+
+
+
+Definition wf_bit_def:
+  wf_bit (bl,len) =
+         (LENGTH bl = len)
+End
+
+
+Definition mk_max_bv_def:
+  mk_max_bv bit_len =
+  (fixwidth bit_len (n2v (max_from_type bit_len)),bit_len)
+End
+           
+Definition mk_min_bv_def:
+  mk_min_bv bit_len =
+  (fixwidth bit_len (n2v 0),bit_len)
+End        
+
+
+
+(*===============================================*)
+(*       convert arith table to interval table   *)
+(*===============================================*)
+
+           
+Definition arith_to_interval_def:
+  arith_to_interval a bit_len =
+    case a of
+    | a_True => SOME (Single (mk_min_bv bit_len) (mk_max_bv bit_len))
+    | a_False => SOME Empty
+    | arithm_ge _ n =>
+        (let (bl,len) = n in
+          if (bit_len = len) ∧ wf_bit n  then
+             SOME (Single n (mk_max_bv bit_len))
+           else
+             NONE)
+          
+    | arithm_le _ n =>
+        (let (bl,len) = n in
+           if (bit_len = len) ∧ wf_bit n then
+              SOME (Single (mk_min_bv bit_len) n)
+            else
+              NONE)
+End
+
+
+
+Definition convert_arith_list_to_interval_def:
+  convert_arith_list_to_interval arith_guards bit_len =
+      MAP (λg. arith_to_interval g bit_len) arith_guards 
+End
+
+        
+Definition convert_arith_rows_to_arith_def:
+  convert_arith_rows_to_arith arith_table bit_len =
+      MAP (λ(arith_guards,st,res). convert_arith_list_to_interval arith_guards bit_len, st, res) arith_table
+End
+
+
+
+
+(*
+still incorrect cause this table blends ttl and src
+EVAL “convert_arith_rows_to_arith
+      [([a_True;
+         arithm_ge (lv_x "ttl") (fixwidth 8 (n2v 1),8);
+         arithm_le (lv_x "src") (fixwidth 8 (n2v 3),8)],1, action "fwd1");
+        
+       ([arithm_ge (lv_x "src") (fixwidth 8 (n2v 4),8)],1,action "fwd2");
+       
+        ([a_True],1,action "drop")] 8”
+
+
+        
+*)
+
+
+
+
+
+Definition valid_line_def:
+  valid_line (guards, s, res) = (guards ≠ [])
+End
+
+
+Definition valid_table_def:
+  valid_table table = 
+    ((table ≠ []) ∧ EVERY valid_line table)
+End
+
+(*
+Definition valid_tables_def:
+  valid_tables tables = EVERY valid_table tables
+End
+*)
+
+        
+
+val _ = Hol_datatype ` 
+  ret_arth_indic = isTrue | isFalse | is_lval of arith_lv
+`;
+      
+
+
+
+
+Definition arth_indic_in_lval_def:
+  arth_indic_in_lval isTrue = F ∧
+  arth_indic_in_lval isFalse = F ∧
+  arth_indic_in_lval (is_lval _) = T           
+End
+
+
+      
+Definition get_lval_from_arith:
+  get_lval_from_arith a_True = isTrue ∧
+  get_lval_from_arith a_False = isFalse ∧
+  get_lval_from_arith (arithm_ge lv _) = is_lval lv ∧
+  get_lval_from_arith (arithm_le lv _) = is_lval lv
+End
+           
+
+
+Definition get_lval_of_ret_arith_list_def:
+  get_lval_of_ret_arith_list ret_arith_guards =
+  let filtered = FILTER (λx. arth_indic_in_lval x) ret_arith_guards in
+    (case nub filtered of
+    | [is_lval lv] => SOME (is_lval lv)
+    | _ => NONE)                           (* if no lval at all after filtering,
+                                              or more than one, then NONE*)
+End
+           
+
+(* this should be for the whole table*)        
+Definition get_lval_of_arith_list_def:
+  get_lval_of_arith_list arith_guards =
+  let lvals = MAP (λarith_g. get_lval_from_arith arith_g) arith_guards in
+        ( case EVERY (λx. ¬ arth_indic_in_lval x) lvals of                (* case all True *)
+          | T => SOME isTrue
+          | F =>
+              ( case get_lval_of_ret_arith_list lvals of     
+                | SOME lv => SOME lv                           (* case blend, return single lval*)
+                | NONE => NONE                                 (* faluty case, shouldn't be reached*)
+              )
+        )
+        
+End
+           
+
+
+
+
+
+(* checks if arithmetic table is convertable to interval table,
+ we do not need to do this as a first step for vars anymore *) 
+Definition analyze_arith_table_type_def:
+  analyze_arith_table_type pd_type arith_table =
+  if valid_table arith_table then
+    let all_guards = FLAT (MAP FST arith_table) in
+      (case get_lval_of_arith_list all_guards of
+       | SOME isFalse => NONE
+       | SOME isTrue => SOME (key_const (n2v 1, 1), 1)
+       | SOME (is_lval lval) =>
+           (case resolve_lval_type pd_type lval of
+            | SOME (type_length n) => SOME (key_val lval, n)
+            | _ => NONE
+           )
+       | NONE => NONE
+      )
+  else
+    NONE
+End
+
+        
+        
+Definition convert_arith_to_interval_table_def:
+  convert_arith_to_interval_table arith_table pd_type =
+  case analyze_arith_table_type pd_type arith_table of
+  | NONE => NONE 
+  | SOME (key, bit_len) =>    
+    (let converted = convert_arith_rows_to_arith arith_table bit_len in
+    if every_is_some_in_l converted ∧ arith_table ≠ [] then
+      SOME ((key, rm_optl converted): 'a intvl_table)
+    else
+      NONE
+    )
+End
+
+
+
+(*
+still incorrect cause this table blends ttl and src
+
+
+val test_pd_type = ``[("h" , type_record [("ttl", type_length 8);
+                                          ("src", type_length 8)])]``;
+                               
+
+                                  
+EVAL “convert_arith_to_interval_table
+      [([   a_True;
+         arithm_ge (lv_acc (lv_x "h") "ttl") (fixwidth 8 (n2v 1),8);
+         arithm_le (lv_acc (lv_x "h") "ttl") (fixwidth 8 (n2v 3),8)],1, action "fwd1");
+        
+       ([arithm_ge (lv_acc (lv_x "h") "ttl") (fixwidth 8 (n2v 4),8)],1,action "fwd2");
+
+       ([a_False],1,action "drop");
+
+        ([a_True],1,action "drop")]
+
+       ^test_pd_type”
+
+
+
+      
+EVAL “convert_arith_to_interval_table
+      [([a_False],1, action "fwd1");
+        
+       ([a_True],1,action "fwd2");
+
+       ([a_False],1,action "drop");
+
+        ([a_False],1,action "drop")]
+
+       ^test_pd_type”
+
+       
+
+        
+*)
+
+
+
+        
+
+
+(*===============================================*)
+(*       sem arith_table = sem interval_table    *)
+(*===============================================*)
+
+(*
+Definition eval_interval_atom_def:
+  (eval_interval_atom arith_lv pd Empty = SOME F) ∧
+  (eval_interval_atom arith_lv pd (Single a b) =
+   (case resolve_lval pd arith_lv of
+    | SOME (val_bs bv) => (
+      case (bv_ge_than bv a, bv_le_than bv b) of
+      | (SOME T, SOME T) => SOME T
+      | (SOME F, SOME _) => SOME F
+      | (SOME _, SOME F) => SOME F
+      | (_,_) => NONE
+      )
+    | _ => NONE
+   )
+  ) 
+End
+*)
+
+
+
+(* bv here could be from the lval in pd or from const*)
+Definition eval_interval_atom_def:
+  (eval_interval_atom bv pd Empty = SOME F) ∧
+  (eval_interval_atom bv pd (Single a b) =
+   case (bv_ge_than bv a, bv_le_than bv b) of
+   | (SOME T, SOME T) => SOME T
+   | (SOME F, SOME _) => SOME F
+   | (SOME _, SOME F) => SOME F
+   | (_,_) => NONE
+  )
+End        
+
+   
+Definition is_interval_guards_true_def:
+  is_interval_guards_true interval_guards bv pd =
+  EVERY (λ interval_atom. eval_interval_atom bv pd interval_atom = SOME T ) interval_guards
+End      
+
+         
+Definition extract_bv_from_key_def:
+  (extract_bv_from_key (key_val lval) pd =
+   case resolve_lval pd lval of
+   | SOME (val_bs bv) => SOME bv
+   | _ => NONE
+  )∧
+  (extract_bv_from_key (key_const bv) pd = SOME bv)
+End
+         
+         
+Definition is_interval_match_row_def:
+  is_interval_match_row st_in st_num artih_atoml bv pd = 
+   ((st_in = st_num) ∧ is_interval_guards_true artih_atoml bv pd ∧ artih_atoml ≠ [])
+End
+
+        
+Definition check_interval_table_sem_def:
+  check_interval_table_sem st_in (interval_table: 'a intvl_table) pd =
+  (let (key, intvl_lines) = interval_table in
+     case (extract_bv_from_key key pd) of
+     | SOME bv =>
+       SOME (MAP (\(interval_guards, st, res).
+         (is_interval_match_row st_in st interval_guards bv pd, res))  intvl_lines)
+     | NONE => NONE
+  )
+End
+
+
+
+Definition match_interval_table_def:
+  match_interval_table st_in (interval_table:'a intvl_table) pd =
+  case check_interval_table_sem st_in interval_table pd of
+    | SOME res =>
+      (case min_idx_till res T of
+        SOME (idx, line) => SOME (SND line)
+       | NONE => NONE
+      )
+    | NONE => NONE
+End
+
+
+(*
+
+
+
+val example_pd =  
+ “([ ("h", val_record [
+            ("ttl", val_bs (fixwidth 8 (n2v 1), (8:num)))
+     ])]): pd”;
+
+
+val example_interval_table=
+ “(key_val (lv_acc (lv_x "h") "ttl"),
+        [([Single ([F; F; F; F; F; F; F; F],8) ([T; T; T; T; T; T; T; T],8);
+           Single ([F; F; F; F; F; F; F; T],8) ([T; T; T; T; T; T; T; T],8);
+           Single ([F; F; F; F; F; F; F; F],8) ([F; F; F; F; F; F; T; T],8)],
+          1,action "fwd1");
+         ([Single ([F; F; F; F; F; T; F; F],8) ([T; T; T; T; T; T; T; T],8)],
+          1,action "fwd2"); ([Empty],1,action "drop");
+         ([Single ([F; F; F; F; F; F; F; F],8) ([T; T; T; T; T; T; T; T],8)],
+          1,action "drop")]): string intvl_table”;
+        
+EVAL “match_interval_table (1:num)
+      ^example_interval_table
+      ^example_pd ”;
+
+*)
+
+
+
+
+
+
+        
+(* questions:
+   1. is this correct or is it way too strong∃
+   2. should it be = instead of implication
+   3. should this to be for all fields of packet or the fields that appear in the policy only?
+ *)
+
+Definition wf_packet_def:
+  wf_packet packet_type packet_input =
+  ∀ lval n.  resolve_lval_type packet_type lval = SOME (type_length n) ⇒
+             ∃ bs. (resolve_lval packet_input lval = SOME (val_bs bs) ∧
+                    wf_bit bs ∧ SND bs = n)
+End
+
+
+
+
+Theorem extract_bv_from_key_not_none:
+  ∀ arith_table packet_type packet_input key rows.        
+    wf_packet packet_type packet_input ∧
+    convert_arith_to_interval_table arith_table packet_type = SOME (key,rows) ⇒
+    extract_bv_from_key key packet_input ≠ NONE
+Proof
+  rw[convert_arith_to_interval_table_def] >>
+  rpt (BasicProvers.FULL_CASE_TAC >> gvs[]) >>
+  gvs[analyze_arith_table_type_def] >>
+  rpt (BasicProvers.FULL_CASE_TAC >> gvs[]) >>
+  gvs[extract_bv_from_key_def] >>
+  rpt (BasicProvers.FULL_CASE_TAC >> gvs[]) >>
+  
+  gvs[wf_packet_def] >>
+  res_tac >> fs[] >>
+  Cases_on ‘resolve_lval packet_input a’ >> gvs[]
+QED
+
+
+
+(*)
+
+
+
+
+        
+
+∀ arith_table interval_table packet_type st_in packet_input.
+wf_packet packet_type packet_input ∧
+convert_arith_to_interval_table arith_table packet_type =
+        SOME interval_table ⇒
+check_interval_table_sem st_in interval_table packet_input = 
+        SOME (check_arith_table_sem st_in arith_table packet_input)
+
+                                    
+rw[check_interval_table_sem_def, check_arith_table_sem_def] >>
+
+Cases_on ‘interval_table’ >> 
+gvs[] >>
+
+Cases_on ‘extract_bv_from_key q packet_input’ >> gvs[] >| [
+    ‘extract_bv_from_key q packet_input ≠ NONE’ by metis_tac[extract_bv_from_key_not_none]
+    ,
+        
+    simp[LIST_EQ_REWRITE] >>
+    ‘LENGTH r = LENGTH arith_table’ by cheat >>
+    gvs[] >>
+
+    rpt strip_tac >>
+    gvs[EL_MAP] >>
+
+    Cases_on ‘EL x' r’ >> Cases_on ‘r'’ >>
+    Cases_on ‘EL x' arith_table’ >> Cases_on ‘r'’ >>
+
+
+    rename1 ‘EL x' r = (interval_guards,interval_st,interval_res)’ >>
+    rename1 ‘EL x' arith_table = (arith_guards,arith_st,arith_res)’ >>
+    gvs[] >>
+
+
+        
+    gvs[convert_arith_to_interval_table_def] >>
+    Cases_on ‘analyze_arith_table_type packet_type arith_table’ >> gvs[] >>
+    Cases_on ‘x''’ >> gvs[] >>
+
+    rename1 ‘i < LENGTH arith_table’ >>
+    rename1 ‘extract_bv_from_key key packet_input = SOME k_val’ >>
+
+    
+            
+
+    
+             
+
+
+
+                                             
+  gvs[every_is_some_in_l_def] >>
+
+
+
+        
+
+
+  ]
+
+
+*)
+                                                        
+
+      
+
+
+
+                                    
+
+
+Theorem table_arith_interval_correct:
+  ∀ arith_table interval_table packet_input packet_type st_in.
+    wf_packet packet_type packet_input ∧
+    (convert_arith_to_interval_table arith_table packet_type = SOME interval_table) ⇒
+    (match_interval_table st_in interval_table packet_input =
+    match_arith_table st_in arith_table packet_input)
+Proof
+  rw[match_interval_table_def, match_arith_table_def] >>
+
+  ‘check_interval_table_sem st_in interval_table packet_input  =
+   SOME (check_arith_table_sem st_in arith_table packet_input) ’ by cheat >>
+  gvs[] 
+QED
+
+        
+
+
+
+(*
+
+
+pd = ["ttl", ([T;T;T], 3)]
+
+ttl >= ([T;F;F;F], 4)
+
+ttl >= ([T;F;F;F], 3)
+   
+
+
+        
+
+        
+OLD STUFF 
+
+
+   
+
+
+        
+Definition intersect_single_def:
+  (intersect_single (SOME (Single bv1 bv2)) (SOME (Single bv3 bv4)) =
+   (if check_widths bv1 bv2 bv3 bv4 then
+     (case (bv_gt_than bv1 bv3, bv_gt_than bv2 bv4) of
+      | (SOME a1_gt_a2, SOME b1_gt_b2) =>
+          (let lower = if a1_gt_a2 then bv1 else bv3 in
+            let upper = if b1_gt_b2 then bv4 else bv2 in
+              (case bv_gt_than lower upper of
+               | SOME F => SOME (Single lower upper)
+               | _ => NONE                (* Shouldn't happen per bv_gt_than spec *)
+              ))
+      | _ => NONE)                        (* Invalid comparison *)
+   else NONE)) ∧                         (* Width/length mismatch *)
+
+        
+  (intersect_single NONE _ = NONE) ∧
+  (intersect_single _ NONE = NONE) ∧
+  (intersect_single (SOME Empty) _ = NONE) ∧
+  (intersect_single _ (SOME Empty) = NONE)
+End
+
+  
+Definition is_True_or_False_def:
+  is_True_or_False g =
+  ((g = True) ∨ (g = False))
+End
+
+     
+Definition process_var_to_arith_def:
+  process_var_to_arith me min max g (SOME curr_int) =
+   case var_atom_to_arith me g of
+   | NONE => NONE                            (* Invalid guard becomes NONE *)
+   | SOME a_True => SOME curr_int            (* True uses full range of the input *)
+   | SOME a_False => NONE                    (* False becomes NONE *)
+   | SOME a => intersect_single (SOME curr_int) (arith_to_interval a min max)
+End
+
+
+(*==================================*)
+(*     line coversion definitions   *)
+(*==================================*)
+
+
+        
+Definition process_guards_rec_def:
+  (process_guards_rec me min max [] init_int = init_int) ∧
+  (process_guards_rec me min max (g::gs) init_int =
+    case init_int of
+    | NONE => NONE
+    | SOME intvl =>
+        case process_var_to_arith me min max g (SOME intvl) of
+        | NONE => NONE
+        | SOME new_intvl => process_guards_rec me min max gs (SOME new_intvl))
+End
+
+        
+Definition convert_line_with_key_def:
+  (convert_line_with_key me min max ([], s, res) = NONE) ∧
+  (convert_line_with_key me min max (var_guards, s, res) =
+    case process_guards_rec me min max var_guards (SOME (Single min max)) of
+    | NONE => SOME (NONE, s, res)  
+    | SOME interval => SOME (SOME interval, s, res))
+End
+
+        
+Definition convert_lines_map_with_key_def:
+  convert_lines_map_with_key me min max lines =
+   MAP (\line.case convert_line_with_key me min max line of
+     | NONE => NONE  (* This is for completely invalid lines *)
+     | SOME x => SOME x   (* Preserve the (interval option, state, action) structure *)) lines
+End
+
+
+
+
+
+(*==================================*)
+(*  WFness conditions for var tbl   *)
+(*==================================*)
+
+
+
+
+Definition all_vars_defined_abstract_def:
+  (all_vars_defined_abstract me [] = T) ∧
+  (all_vars_defined_abstract me (True::rest) = all_vars_defined_abstract me rest) ∧
+  (all_vars_defined_abstract me (False::rest) = all_vars_defined_abstract me rest) ∧
+  (all_vars_defined_abstract me ((Var x)::rest) = 
+   (case ALOOKUP me x of
+     | SOME _ => all_vars_defined_abstract me rest
+     | NONE => F)) ∧
+  (all_vars_defined_abstract me ((Not g)::rest) = 
+   (all_vars_defined_abstract me [g] ∧ all_vars_defined_abstract me rest))
+End
+
+
+
+
+
+
+Definition get_lval_of_guard_in_me_def:
+  get_lval_of_guard_in_me me var_g = 
+    case var_g of
+      | Var x => (case ALOOKUP me x of
+                  | SOME a => get_lval a
+                  | NONE => NONE)
+      | Not (Var x) => (case ALOOKUP me x of
+                        | SOME a => get_lval a
+                        | NONE => NONE)
+      | _ => NONE
+End
+
+
+Definition get_guard_lvals_def:
+  get_guard_lvals me guards = 
+    FILTER (λ x . IS_SOME x ) (MAP (get_lval_of_guard_in_me me) guards)
+End
+
+
+Definition ALL_SAME_def:
+  (ALL_SAME [] = T) ∧
+  (ALL_SAME [x] = T) ∧
+  (ALL_SAME (x::y::rest) = ((x = y) ∧ ALL_SAME (y::rest)))
+End
+
+
+Definition one_unique_lval_in_guards_def:
+  one_unique_lval_in_guards me all_guards =
+    let lvals = get_guard_lvals me all_guards in
+    case lvals of
+      | [] => NONE   (* No lvals found *)
+      | h::t => if ALL_SAME (h::t) 
+                then h  (* Returns SOME lv if all same *)
+                else NONE
+End      
+
+       
+Definition valid_line_def:
+  valid_line (guards, s, res) = (guards ≠ [])
+End
+
+
+Definition valid_table_def:
+  valid_table table = 
+    ((table ≠ []) ∧ EVERY valid_line table)
+End
+
+
+Definition valid_tables_def:
+  valid_tables tables = EVERY valid_table tables
+End
+
+  
+
+(* Add this new function to analyze the entire table first *)
+Definition analyze_table_type_def:
+  analyze_table_type me pd_type table =
+   if table = [] then NONE else 
+     let all_guards = FLAT (MAP FST table) in
+       case all_vars_defined_abstract me all_guards  of
+       | T => ( case EVERY (λx. x = (False:atom_var)) all_guards of
+                | T => NONE
+                | F =>  (case EVERY (λx. x = True) all_guards of
+                         | T => SOME (T, key_const (n2v 1, 1), (n2v 0,1), (n2v 1,1))
+                         | F => ( case one_unique_lval_in_guards me all_guards of
+                                  (* All non-boolean guards use same lval *)
+                                  | SOME lv => (
+                                    case resolve_pd_min_max pd_type lv of
+                                    | SOME (min,max) => SOME (T, key_val lv, min, max)
+                                    | NONE => NONE
+                                    )
+                                  | NONE => NONE
+                                )
+                        )
+              )
+       | F => NONE 
+End
+
+
+(*==================================*)
+(*         Tables conversion        *)
+(*==================================*)
+
+Definition convert_single_table_def: 
+  (convert_single_table [] me pd_type = NONE) ∧
+  (convert_single_table lines me pd_type =                
+   case analyze_table_type me pd_type lines of
+   | SOME (T, key_type, min, max) =>       
+       let converted_lines = convert_lines_map_with_key me min max lines in
+         if EVERY IS_SOME converted_lines then
+           SOME (key_type, MAP THE converted_lines)  (* All lines valid *)
+         else
+           NONE  (* At least one line was completely invalid (NONE) *)
+   | _ => NONE  (* Inconsistent table *)
+  )
+End
+
+        
+Definition convert_tables_def:
+  (convert_tables [] _ _ = SOME []) ∧
+  (convert_tables (tbl::tbls) me pd_type =
+    if ¬(valid_tables (tbl::tbls)) then NONE
+      else
+        (case convert_single_table tbl me pd_type of
+        | NONE => NONE  (* Fail immediately if any table fails *)
+        | SOME converted_tbl =>
+            (case convert_tables tbls me pd_type of
+            | NONE => NONE
+            | SOME converted_tbls => SOME (converted_tbl :: converted_tbls))
+        )
+      )
+End
+
+
+
+(*
+val policy1_var = “[[([(Var "x" :atom_var); (Var "y" :atom_var)],(0 :num), (state (3 :num) :(string # num list) action_expr));
+       ([(Var "x" :atom_var); Not (Var "y" :atom_var)],(0 :num), (state (4 :num) :(string # num list) action_expr));
+       ([Not (Var "x" :atom_var)],(0 :num),                      (state (4 :num) :(string # num list) action_expr))];
+       
+      [([(Var "z" :atom_var)],(4 :num),                          (state (7 :num) :(string # num list) action_expr));
+       ([Not (Var "z" :atom_var)],(4 :num),                      (state (8 :num) :(string # num list) action_expr));
+       ([True],(3 :num),                                         (state (3 :num) :(string # num list) action_expr))];
+       
+      [([True],(3 :num),action ("fwd",[(1 :num)]));
+       ([True],(7 :num),action ("fwd",[(2 :num)]));
+       ([True],(8 :num),action ("drop",([] :num list)))]]”;
+
+
+val test_pd_nested = ``[
+  ("h", type_record [
+    ("len", type_length 5); 
+    ("flags", type_length 5); 
+    ("ttl", type_length 5)
+  ])
+]``;
+
+
+val test_lval1 = ``lv_acc (lv_x "h") "ttl"``;
+val test_lval2 = ``lv_acc (lv_x "h") "flags"``;
+val test_lval3 = ``lv_x "z"``;
+
+
+val test_atom1 = ``arithm_gt ^test_lval1 (n2v 0,5)``;  (* h.ttl > 0 *)
+val test_atom2 = ``arithm_lt ^test_lval1 (n2v 10,5)``; (* h.ttl < 10 *)
+val test_atom3 = ``arithm_lt ^test_lval2 (n2v 3,5)``;  (* h.flags < 3 *)
+
+    
+val test_me = ``[
+  ("x", ^test_atom1); 
+  ("y", ^test_atom2); 
+  ("z", ^test_atom3)
+]``;
+
+EVAL ``convert_tables (^policy1_var) ^test_me ^test_pd_nested``;
+        
+*)
+
+
+
+                  
+
+(*==================================*)
+(*    interval table semantics      *)
+(*==================================*)
+
+
+
+
+Definition is_intvl_match_row_def:
+  is_intvl_match_row key (s_in:num) (packet_input:pd) (row:('a intvl_row)) =
+  case (key, row) of
+  | (key_val lval, (SOME (Single a b), s, res)) =>
+      (let (a_v,a_w) = a in
+        let (b_v,b_w) = b in
+          (case resolve_lval packet_input lval of
+           | SOME (val_bs (v,v_w)) => 
+               (if (a_w = b_w) ∧ (b_w = v_w) then
+                  (case (bv_lt_than (v,v_w) (a_v,a_w), bv_lt_than (b_v,b_w) (v,v_w)) of
+                   | (SOME F, SOME F) => (s_in = s)  (* a ≤ v ≤ b *)
+                   | _ => F)
+                else F
+               )
+           | SOME _ => F  (* non-numeric value *)
+           | NONE => F))   (* lval not found *)
+  | (key_val lval, (NONE, s, res)) => F  (* Empty interval never matches *)             
+  | (key_const (c,c_w), (_, s, _)) => (s_in = s)  (* Constant key matches state only *)
+End
+
+      
+        
+
+(* Process all rows in an interval table *)
+Definition check_all_intvl_rows_match_def:
+  check_all_intvl_rows_match key st_in rows packet_input =
+  MAP (λ(interval,s,res). is_intvl_match_row key (st_in:num) (packet_input:pd) (interval,s,res), res) rows
+End
+
+
+
+(* Find first matching line in a converted table *)
+Definition match_intvl_tbl_def:
+  match_intvl_tbl (intvl_tbl: 'a intvl_table) packet_input st_in =
+  let (key, rows) = intvl_tbl in
+    let lines_res = check_all_intvl_rows_match key st_in rows packet_input in
+      case min_idx_till lines_res T of
+      | SOME (idx, line) => SOME (SND line)
+      | NONE => NONE
+End
+
+
+(* Process list of interval tables with state propagation *)
+Definition match_intvl_tbll_def:
+  (match_intvl_tbll ([]: 'a intvl_table_list) packet_input st_in = NONE) ∧
+  (match_intvl_tbll [intvl_tbl] packet_input st_in =
+    case match_intvl_tbl intvl_tbl packet_input st_in of
+      | SOME (action a) => SOME (action a)
+      | _ => NONE) ∧
+  (match_intvl_tbll (intvl_tbl::intvl_tbls) packet_input st_in =
+    case match_intvl_tbl intvl_tbl packet_input st_in of
+      | SOME (state n) => match_intvl_tbll intvl_tbls packet_input n
+      | _ => NONE)
+End
+
+
+
+(* Top-level interval table semantics *)
+Definition sem_intvl_tables_def:
+  sem_intvl_tables ((intvl_tbll: (('a intvl_table ) list)), st_in) (packet_input:pd) =
+  match_intvl_tbll intvl_tbll packet_input st_in
+End
+
+(* IMPORTANT well formdness every var in me is indeed defined in pd*)
+
+
+
+
+        
+
+(*==================================*)
+(*            P R O O F             *)
+(*==================================*)
+
+
+
+
+
+Theorem convert_tables_never_empty:
+  ∀ h' t me packet_type.
+    convert_tables (h'::t) me packet_type ≠ SOME []
+Proof
+  rw[convert_tables_def] >>
+  rpt (BasicProvers.FULL_CASE_TAC >> gvs[]) 
+QED
+   
+
+Theorem append_defined_implies_first_defined:
+  ∀me l l'. all_vars_defined_abstract me (l ++ l') ⇒
+              (all_vars_defined_abstract me l' ∧  all_vars_defined_abstract me l)
+Proof
+  Induct_on `l` >> simp[all_vars_defined_abstract_def] >>
+  Cases >> simp[all_vars_defined_abstract_def] >>
+  rpt strip_tac >> res_tac >>
+  rpt (BasicProvers.FULL_CASE_TAC >> gvs[]) >> 
+  res_tac
+QED
+
+
+
+Theorem check_all_rows_match_length:
+  ∀ tbl mv st_in.
+    LENGTH (check_all_rows_match st_in tbl mv) = LENGTH (tbl)
+Proof
+  Induct >>
+  gvs[check_all_rows_match_def]
+QED
+
+
+Theorem convert_lines_map_with_key_length:
+  ∀ tbl me min max.
+    LENGTH (convert_lines_map_with_key me min max tbl) = LENGTH tbl
+Proof
+  Induct >>
+  gvs[convert_lines_map_with_key_def]
+QED
+
+
+Theorem check_all_intvl_rows_match_comb_length:
+  ∀ tbl me min max key st_in packet_input.
+    LENGTH (check_all_intvl_rows_match key st_in (MAP THE (convert_lines_map_with_key me min max tbl)) packet_input) =
+    LENGTH tbl
+Proof
+  Induct >>
+  gvs[check_all_intvl_rows_match_def, convert_lines_map_with_key_def]
+QED
+
+
+
+
+Theorem guards_in_tbl_not_empty:
+  ∀ tbl x guards st_row res_row.
+  valid_table tbl ∧
+  x < LENGTH tbl ∧
+  EL x tbl = (guards,st_row,res_row) ⇒
+  guards ≠ []      
+Proof
+  rw[valid_table_def, EVERY_EL, valid_line_def] >>
+  res_tac >>
+  metis_tac[valid_line_def]           
+QED
+        
+
+
+
+Theorem all_rows_true_then_lval_none_thm:
+  ∀ rows snlist me.
+    EVERY (λx. x = True) rows ∧
+    FILTER (λx. IS_SOME x) (MAP (get_lval_of_guard_in_me me) rows) = snlist ⇒
+    EVERY IS_NONE  snlist
+Proof
+  Induct >>
+  rpt strip_tac >>
+  gvs[] >>
+  rpt (BasicProvers.FULL_CASE_TAC >> rgs[]) >>
+  gvs[get_lval_of_guard_in_me_def]
+QED
+    
+        
+        
+Theorem every_true_then_in_mv_true_l_thm:
+  ∀ row st res mv x tbl.
+    x < LENGTH tbl ∧
+    EL x tbl = (row,st,res) ∧
+    EVERY (λx. x = True) (FLAT (MAP FST tbl)) ⇒
+    is_atoml_true row mv
+Proof
+  rw[is_atoml_true_def] >>
+  imp_res_tac EL_MEM >>           
+  gvs[EVERY_MEM] >>
+  rpt strip_tac >>
+  imp_res_tac mem_fst_snd >>
+  gvs[MEM_FLAT] >>
+  res_tac >>
+  gvs[sem_var_atom_def]
+QED
+
+        
+Theorem all_rows_true_then_no_unique:
+  ∀ rows me.
+    EVERY (λx. x = True) rows ⇒             
+    one_unique_lval_in_guards me rows = NONE
+Proof
+  
+  gvs[one_unique_lval_in_guards_def] >>                            
+  gvs[get_guard_lvals_def, get_lval_of_guard_in_me_def] >>
+  rpt strip_tac >>
+  rpt (BasicProvers.FULL_CASE_TAC >> rgs[]) >>
+  imp_res_tac all_rows_true_then_lval_none_thm >>
+  gvs[]
+QED
+  
+
+
+        
+        
+Theorem  all_vars_defined_abstract_on_individual:       
+  ∀ me  l.    
+    (all_vars_defined_abstract me) (FLAT l) ⇒
+    (EVERY (\x. all_vars_defined_abstract me x) l)
+Proof
+  Induct_on `l` >> simp[all_vars_defined_abstract_def] >>
+  Cases >> simp[all_vars_defined_abstract_def] >>
+  rpt strip_tac >> res_tac >>
+  `h'::(t ++ FLAT l) = [h'] ++ t ++ FLAT l` by simp[] >> 
+  `(h':: t) = [h'] ++ t ` by simp[] >> 
+  metis_tac[append_defined_implies_first_defined]
+QED
+
+
+
+
+
+
+        
+Definition norm_match_tbl_def:
+  (norm_match_tbl [] mv st_in = NONE) ∧
+  (norm_match_tbl (h::t) mv st_in =
+   let (guards,st,res) = h in
+    if is_match_row st_in st guards mv then
+      SOME res
+    else
+      norm_match_tbl t mv st_in)
+End
+
+
+Theorem norm_match_tbl_equiv:
+  ∀tbl mv st_in.
+    norm_match_tbl tbl mv st_in = match_tbl tbl mv st_in
+Proof
+  Induct >> rw[] >-
+  (
+  fs[norm_match_tbl_def, match_tbl_def, check_all_rows_match_def, min_idx_till_def, INDEX_FIND_def]
+  ) >>
+  PairCases_on ‘h’ >>
+  fs[norm_match_tbl_def, match_tbl_def, check_all_rows_match_def] >>
+  Cases_on `is_match_row st_in h1 h0 mv` >> fs[] >>
+  gvs[min_idx_till_def, INDEX_FIND_def] >>
+  rpt (BasicProvers.FULL_CASE_TAC >> gvs[]) >>  
+
+  imp_res_tac INDEX_FIND_NONE_EXISTS >>
+  imp_res_tac exists_index_some >>
+  gvs[EXISTS_MAP] >>
+  gvs[MAP_MAP_o] >>          
+  imp_res_tac P_implies_next >>
+  gvs[]     
+QED
+
+
+
+
+
+Theorem all_vars_defined_abstract_normalize:
+  ∀ h guards me.
+    all_vars_defined_abstract me (h::guards) ⇒
+    all_vars_defined_abstract me [h] ∧
+    all_vars_defined_abstract me guards
+Proof
+  Cases_on ‘h’ >>                          
+  rw[all_vars_defined_abstract_def] >>
+  rpt (BasicProvers.FULL_CASE_TAC >> gvs[])
+QED
+
+Theorem check_intvl_rows_elementwise_correct:
+  ∀l key st_in packet_input x x'.
+    x < LENGTH l ∧
+    EL x l = SOME x' ⇒
+    (EL x (check_all_intvl_rows_match key st_in (MAP THE l) packet_input) =
+     HD (check_all_intvl_rows_match key st_in [x'] packet_input))
+Proof
+  rpt gen_tac >> strip_tac >>
+  (* Expand both sides *)
+  simp[check_all_intvl_rows_match_def] >>
+  gvs[EL_MAP]                              
+QED
+
+
+Triviality unique_lval_gt_same_triv1:
+  ∀ var guards lval lval' me p.
+    one_unique_lval_in_guards me (Var var::guards) = SOME lval ∧
+    ALOOKUP me var = SOME (arithm_gt lval' p) ⇒
+    lval = lval'
+Proof
+  rw[one_unique_lval_in_guards_def] >>
+  gvs[get_guard_lvals_def] >>
+  gvs[get_lval_of_guard_in_me_def] >>
+  rpt (BasicProvers.FULL_CASE_TAC >> gvs[]) >>
+  gvs[get_lval_def]
+QED
+
+
+
+
+Triviality unique_lval_lt_same_triv1:
+  ∀ var guards lval lval' me p.
+    one_unique_lval_in_guards me (Var var::guards) = SOME lval ∧
+    ALOOKUP me var = SOME (arithm_lt lval' p) ⇒
+    lval = lval'
+Proof
+  rw[one_unique_lval_in_guards_def] >>
+  gvs[get_guard_lvals_def] >>
+  gvs[get_lval_of_guard_in_me_def] >>
+  rpt (BasicProvers.FULL_CASE_TAC >> gvs[]) >>
+  gvs[get_lval_def]
+QED
+
+
+
+
+
+
+
+
+        
+
+
+
+  
+        
+        
+(*******************************************************)
+
+
+
+
+
+
+
+
+
+
+
+
+        
+
+        
+Theorem el_rows_match_check_thm:
+  ∀me mv packet_input packet_type  st_in tbl x interval st res key min max.
+    ALL_DISTINCT (MAP FST me) ∧
+    valid_table tbl ∧
+    (∀var atom.
+       ALOOKUP me var = SOME atom ⇒
+       ALOOKUP mv var = eval_arithm_atom packet_input atom) ∧
+    analyze_table_type me packet_type tbl = SOME (T,key,min,max) ∧ 
+    LENGTH (convert_lines_map_with_key me min max tbl) =
+    LENGTH (check_all_rows_match st_in tbl mv) ∧
+    EL x (convert_lines_map_with_key me min max tbl) =
+    SOME (interval,st,res) ∧
+    x < LENGTH (check_all_rows_match st_in tbl mv)
+    ⇒
+    EL x (check_all_rows_match st_in tbl mv) =
+    (is_intvl_match_row key st_in packet_input (interval,st,res),res)
+Proof
+
+  rpt gen_tac >> strip_tac >>
+  fs[convert_lines_map_with_key_def, check_all_rows_match_def] >>
+  gvs[] >>
+  
+  Cases_on ‘EL x tbl’ >>   Cases_on ‘r’ >>
+  rename1 ‘EL x tbl = (guards, st_row, res_row)’ >>
+  
+  gvs[EL_MAP] >>
+  
+  rpt (BasicProvers.FULL_CASE_TAC >> gvs[]) >>
+
+  ‘guards ≠ []’ by metis_tac[guards_in_tbl_not_empty] >>
+
+  Cases_on ‘key’ >|[
+    (* Case 1: key_val *)
+    rgs[analyze_table_type_def] >>
+    rpt (BasicProvers.FULL_CASE_TAC >> rgs[]) >>  
+    gvs[] >>
+    
+    (* we check if the row contains at least one lval or not *)
+    Cases_on ‘one_unique_lval_in_guards me guards’ >> gvs[] >|[
+      (* if not, trivial,  all values are true and false or not defined (by contrdiction)*)
+      cheat
+      ,
+      
+      (* else this lval will be the same for the whole table *)
+      ‘a=x'’ by cheat >>
+      Cases_on ‘guards’ >> gvs[] >>
+      
+      gvs[convert_line_with_key_def] >>
+      Cases_on ‘process_guards_rec me min max (h::t) (SOME (Single min max))’ >> gvs[] >|[
+          
+          simp[is_match_row_def, is_intvl_match_row_def] >>
+          strip_tac >>
+          ‘all_vars_defined_abstract me (h::t)’ by cheat >>  (* trivial from condition *)
+          irule none_interval_implies_false_guard >>
+          qexistsl_tac [‘a’, ‘max’, ‘me’, ‘min’, ‘packet_input’, ‘packet_type’] >>
+          gvs[]
+          ,
+          (*process retunrs some*)
+          
+          
+        ]
+    ,
+    (* Case 2: key_const *)
+    rgs[analyze_table_type_def] >>
+    rpt (BasicProvers.FULL_CASE_TAC >> rgs[]) >>
+    imp_res_tac all_rows_true_then_no_unique >>
+    gvs[] >>
+    
+    Cases_on ‘guards’ >> gvs[convert_line_with_key_def] >>
+    rpt (BasicProvers.FULL_CASE_TAC >> gvs[]) >>  
+    
+    gvs[is_match_row_def, is_intvl_match_row_def] >>
+    ‘is_atoml_true (h::t) mv’ by metis_tac[every_true_then_in_mv_true_l_thm] >> gvs[]
+                                                                                   
+  ]
+
+QED
+
+
+
+
+Theorem interval_all_rows_converstion_correctness:
+  ∀ tbl me packet_input mv packet_type st_in key min max.
+    ALL_DISTINCT (MAP FST me) ∧
+    valid_table tbl ∧
+    (∀var atom.
+       ALOOKUP me var = SOME atom ⇒
+       ALOOKUP mv var = eval_arithm_atom packet_input atom) ∧
+    EVERY IS_SOME (convert_lines_map_with_key me min max (tbl)) ∧
+    analyze_table_type me packet_type tbl = SOME (T,key,min,max) ⇒
+    ((check_all_rows_match st_in tbl mv) =
+     (check_all_intvl_rows_match key st_in (MAP THE (convert_lines_map_with_key me min max tbl)) packet_input))
+Proof
+  rw[LIST_EQ_REWRITE] >|[
+    
+    ‘LENGTH (check_all_rows_match st_in tbl mv) = LENGTH (tbl)’ by gvs[check_all_rows_match_length] >>
+    ‘LENGTH (convert_lines_map_with_key me min max tbl) = LENGTH tbl’ by gvs[convert_lines_map_with_key_length] >>
+    gvs[check_all_intvl_rows_match_comb_length]
+    ,
+
+
+    ‘LENGTH (convert_lines_map_with_key me min max tbl) =
+     LENGTH (check_all_rows_match st_in tbl mv)’ by gvs[check_all_rows_match_length, convert_lines_map_with_key_length] >>
+    gvs[EVERY_EL] >>
+    
+    first_x_assum (strip_assume_tac o (Q.SPECL [‘x’])) >>
+    res_tac >>
+
+    Cases_on ‘EL x (convert_lines_map_with_key me min max tbl)’ >> rw[IS_SOME_DEF] >> gvs[] >>
+
+    imp_res_tac check_intvl_rows_elementwise_correct >>
+    ‘x < LENGTH (convert_lines_map_with_key me min max tbl)’ by gvs[] >>
+    res_tac >>
+                                                                                          
+    first_x_assum (strip_assume_tac o (Q.SPECL [‘st_in’, ‘packet_input’, ‘key’])) >>
+    res_tac >>
+                                        
+    gvs[] >>
+
+    gvs[check_all_intvl_rows_match_def] >>
+    PairCases_on ‘x'’ >>
+    gvs[] >>
+
+    rename1 ‘EL x (convert_lines_map_with_key me min max tbl) = SOME (interval,st,res)’ >>
+    imp_res_tac  el_rows_match_check_thm (* theorem here*)
+  ]
+QED
+
+
+      
+Theorem interval_single_table_converstion_correctness:
+  ∀var_table me packet_input mv interval_table packet_type st_in.
+    ALL_DISTINCT (MAP FST me) ∧
+    valid_table var_table  ∧
+    (∀var atom.  ALOOKUP me var = SOME atom ⇒
+                 ALOOKUP mv var = eval_arithm_atom packet_input atom) ∧
+    convert_single_table var_table me packet_type = SOME interval_table ⇒
+    match_tbl var_table mv st_in = match_intvl_tbl interval_table packet_input st_in
+Proof
+  
+  Cases_on ‘var_table’ >>
+  rpt strip_tac >-
+   gvs[valid_table_def] >>
+  
+  gvs[convert_single_table_def] >>
+  rpt (BasicProvers.FULL_CASE_TAC >> gvs[]) >>  
+  
+  rename1 ‘analyze_table_type me packet_type (row::tbl) = SOME (T,key,min,max)’ >>
+  gvs[match_tbl_def, match_intvl_tbl_def] >>
+  
+  ‘(check_all_rows_match st_in (row::tbl) mv) = (check_all_intvl_rows_match key st_in
+               (MAP THE (convert_lines_map_with_key me min max (row::tbl)))
+               packet_input)’ by metis_tac[interval_all_rows_converstion_correctness] >>    (* thm here *)
+  
+  gvs[]
+QED
+
+        
+
+        
+Theorem interval_tables_conversion_correctness:
+  ∀var_tables me packet_input mv interval_tables packet_type st_in.
+    ALL_DISTINCT (MAP FST me) ∧
+    (∀var atom. 
+       ALOOKUP me var = SOME atom ⇒ 
+       ALOOKUP mv var = eval_arithm_atom packet_input atom) ∧
+    (convert_tables var_tables me packet_type = SOME interval_tables) ⇒
+    sem_tables (var_tables, st_in) mv = 
+    sem_intvl_tables (interval_tables, st_in) packet_input
+Proof
+  Induct >> rpt strip_tac >-
+   
+   (fs[convert_tables_def, sem_tables_def, sem_intvl_tables_def] >>
+    gvs[sem_tables_def, match_tbll_def, sem_intvl_tables_def, match_intvl_tbll_def]) >> 
+  
+  fs[convert_tables_def] >>     
+  Cases_on ‘convert_single_table h me packet_type’ >> fs[] >>
+  Cases_on ‘convert_tables var_tables me packet_type’ >> fs[] >>
+  
+  last_x_assum (drule_all_then strip_assume_tac) >>
+  gvs[] >>
+  
+
+  ‘valid_table h’ by gvs[valid_tables_def] >>
+        
+  subgoal ‘match_tbl h mv st_in = match_intvl_tbl x packet_input st_in’ >-
+   ( metis_tac[interval_single_table_converstion_correctness] ) >>                 (*thm here*)
+  
+  simp[sem_tables_def, sem_intvl_tables_def] >>
+  
+  Cases_on ‘var_tables’ >>
+  Cases_on ‘x'’ >>
+  gvs[] >|[
+    (* both are last tables*)
+    fs[match_tbll_def, match_intvl_tbll_def] 
+    ,
+    fs[convert_tables_def]
+    ,
+    gvs[convert_tables_never_empty]
+    ,
+    fs[match_tbll_def, match_intvl_tbll_def] >>
+    rpt (BasicProvers.FULL_CASE_TAC >> gvs[]) >>
+    fs[sem_tables_def, sem_intvl_tables_def] 
+  ]   
+QED
+
+
+
+
+
+
+
+
+*)
+        
+   
+
+
+                                                                
+
+val _ = export_theory ();
+
+
+
+
+
+
+
