hol/table_bs_propertiesScript.sml
@@ -1,0 +1,531 @@
+open HolKernel boolLib liteLib simpLib Parse bossLib;
+open arithmeticTheory stringTheory containerTheory pred_setTheory
+     listTheory finite_mapTheory;
+
+open p4Lib;
+open blastLib bitstringLib;
+open p4Theory;
+open p4_auxTheory;
+open p4_coreTheory;
+
+open bitstringTheory;
+open wordsTheory;
+open optionTheory;
+open sumTheory;
+open stringTheory;
+open ottTheory;
+open pairTheory;
+open rich_listTheory;
+open arithmeticTheory;
+open alistTheory;
+open numeralTheory;
+open alistTheory;
+open pred_setTheory;
+open pred_setLib;
+  
+
+
+val _ = new_theory "table_bs_properties";
+
+Definition max_from_type_def:
+  max_from_type type =
+  (2:num) ** type - (1:num)
+End
+
+
+Theorem bitv_binpred_same_length:
+  ∀ binop_any bv1 bv2 x.
+    bitv_binpred binop_any bv1 bv2 = SOME x ⇒
+    (SND bv1 = SND bv2)
+Proof
+  rpt gen_tac >>
+  PairCases_on ‘bv1’ >>
+  PairCases_on ‘bv2’ >>
+  
+  RW.ONCE_RW_TAC [bitv_binpred_def] >>
+  gvs[]
+QED
+
+
+Theorem bitv_binpred_range_length:
+  ∀ binop_any bv1 bv2 x.
+    bitv_binpred binop_any bv1 bv2 = SOME x ⇒
+    (SND bv1 > 0 ∧ SND bv1 < 129)
+Proof
+  rpt gen_tac >>
+  PairCases_on ‘bv1’ >>
+  PairCases_on ‘bv2’ >>
+  
+  RW.ONCE_RW_TAC [bitv_binpred_def] >>
+  gvs[] >>
+
+  RW.ONCE_RW_TAC [bitv_binpred_inner_def] >>
+  rpt strip_tac >>
+      
+  rpt(
+    BasicProvers.FULL_CASE_TAC >-
+     (fs[] >>
+      intLib.COOPER_TAC
+     )) >>
+  intLib.COOPER_TAC 
+QED
+
+        
+Theorem bitv_binop_range_length:
+  ∀ binop_any bv1 bv2 bv3.
+    (SND bv2 > 0 ∧ SND bv2 < 129) ∧
+    bitv_binop binop_any bv1 bv2 = SOME bv3 ⇒
+    (SND bv3 = SND bv2)
+Proof
+  rpt gen_tac >>
+  PairCases_on ‘bv1’ >>
+  PairCases_on ‘bv2’ >>
+  PairCases_on ‘bv3’ >>
+  
+  RW.ONCE_RW_TAC [bitv_binop_def] >>
+  gvs[] >>
+
+  RW.ONCE_RW_TAC [bitv_binop_inner_def] >>
+  rpt strip_tac >>
+      
+  rpt (
+    BasicProvers.FULL_CASE_TAC >-
+     fs[]
+    ) >>
+  intLib.COOPER_TAC 
+QED
+
+
+Theorem all_bs_larger_than_zero:
+  ∀ bl len.
+    len > 0 ∧ len < 129 ⇒
+    bitv_binpred binop_ge (bl,len) (fixwidth len (n2v 0),len) = SOME T
+Proof                                   
+  RW.ONCE_RW_TAC [bitv_binpred_def] >>
+  rpt strip_tac >>
+  gvs[] >>
+  
+  RW.ONCE_RW_TAC [bitv_binpred_inner_def] >>
+
+  rpt (
+    BasicProvers.FULL_CASE_TAC >-                         
+     (gvs[] >>
+      gvs[get_word_binpred_def] >>
+      EVAL_TAC
+     )
+    ) >> intLib.COOPER_TAC
+QED
+
+        
+
+Triviality v2w_zero_eq1:
+  v2w (fixwidth 128 (n2v 0)) = (0w : word128) 
+Proof
+  EVAL_TAC
+QED
+
+
+Theorem fixed_width_imp_v_words_zero:
+  ∀ n.
+    n = fixwidth 128 (n2v 0) ⇒ v2w n = (0w : word128) 
+Proof
+  blastLib.FULL_BBLAST_TAC >>
+  EVAL_TAC >>
+  gvs[]
+QED
+
+
+
+
+(* theorem of
+   fixwidth 128 bl = fixwidth 128 (n2v 0) ⇒ (v2w bl: word128 word) = v2w (n2v 0)
+   ...
+   fixwidth 1 bl   = fixwidth 1   (n2v 0) ⇒ (v2w bl: word1 word) = v2w (n2v 0)
+*)
+        
+fun gen_fixwidth_thm len = let
+  val len_term = numSyntax.term_of_int len
+  val word_ty = wordsSyntax.mk_int_word_type len
+  val bl_var = mk_var("bl", Type`:bitstring`)
+                   
+  val lhs = bitstringSyntax.mk_v2w(bl_var, fcpSyntax.mk_int_numeric_type len) 
+  val rhs = bitstringSyntax.mk_v2w(“n2v 0”, fcpSyntax.mk_int_numeric_type len)
+                  
+  val premise1 = bitstringSyntax.mk_fixwidth(len_term, bl_var)
+  val premise2 = bitstringSyntax.mk_fixwidth(len_term, “n2v 0”)
+                              
+  val eq = mk_eq(lhs, rhs)
+  val premise = mk_eq(premise1,premise2)
+  val imp = mk_imp(premise, eq)
+  val goal = list_mk_forall([bl_var], imp)
+                                                
+  val thm = prove(goal,gvs[v2w_11] )
+
+in
+    thm
+end;
+
+
+val all_fixwidth_thms = List.tabulate(128, fn i => gen_fixwidth_thm (i+1));            
+val big_thm = LIST_CONJ all_fixwidth_thms;
+val fixwidth_zero_all_thm = save_thm("fixwidth_zero_all", big_thm);
+
+
+
+
+(* takes forever *)
+Theorem all_bs_larger_than_zero2:
+  ∀ len bl bl'.
+    len > 0 ∧ len < 129 ∧
+    fixwidth len bl' = fixwidth len (n2v 0) ⇒
+    bitv_binpred binop_ge (bl,len) (bl',len) = SOME T
+Proof                                           
+  RW.ONCE_RW_TAC [bitv_binpred_def] >>
+  rpt strip_tac >>
+  gvs[] >>
+  
+  RW.ONCE_RW_TAC [bitv_binpred_inner_def] >>
+  
+  rpt
+  (
+  BasicProvers.FULL_CASE_TAC >-
+   (                           
+   gvs[] >>
+   gvs[get_word_binpred_def] >>
+   
+   imp_res_tac fixwidth_zero_all_thm >>
+   gvs[] >>
+   blastLib.FULL_BBLAST_TAC        
+   ) 
+  ) >>
+  intLib.COOPER_TAC
+QED
+
+                         
+
+
+(* theorem of
+   (∀a b. a ≠ 0w ⇒ (b ≤₊ a − 1w ⇔ ¬(b ≥₊ a)))
+*)
+
+  
+fun gen_word_ineq_thm len = let
+    val word_ty = wordsSyntax.mk_int_word_type len
+    val a = mk_var("a", word_ty)
+    val b = mk_var("b", word_ty)
+    val zero = wordsSyntax.mk_wordii (0, len)
+                                     
+    val premise = mk_neg(mk_eq(a, zero))
+    val le_expr = wordsSyntax.mk_word_ls(b, 
+                       wordsSyntax.mk_word_sub(a, wordsSyntax.mk_wordii (1, len)))
+    val ge_expr = wordsSyntax.mk_word_hs(b, a)
+    val conclusion = mk_eq(le_expr, mk_neg ge_expr)
+    val goal = list_mk_forall([a, b], mk_imp(premise, conclusion))
+in
+    prove(goal, rpt strip_tac >> blastLib.FULL_BBLAST_TAC )
+end;
+
+val word_ineq_thms = List.tabulate(128, fn i => gen_word_ineq_thm (i+1));
+val word_ineq_all1 = LIST_CONJ word_ineq_thms;
+val word_ineq_all1_thm = save_thm("word_ineq_all_sizes", word_ineq_all1);
+
+
+
+
+    
+(*
+
+fixwidth 128 n ≠ fixwidth 128 (n2v 0) ⇒
+       (v2w lval_bl ≤₊ v2w n − 1w ⇔ ¬(v2w lval_bl ≥₊ v2w n)
+*)
+
+fun prove_ineq2_thm len = let
+
+  val word_ty = wordsSyntax.mk_int_word_type len
+  val size_term = numSyntax.term_of_int len
+  val n_var = mk_var("n", ``:bitstring``)
+  val lval_var = mk_var("lval_bl", ``:bitstring``)
+  
+  val fixwidth_n = bitstringSyntax.mk_fixwidth(size_term, n_var)
+  val fixwidth_0 = bitstringSyntax.mk_fixwidth(size_term, “n2v 0”)
+                                                        
+  val v2w_n = bitstringSyntax.mk_v2w(n_var, fcpSyntax.mk_int_numeric_type len)
+  val v2w_l = bitstringSyntax.mk_v2w(lval_var, fcpSyntax.mk_int_numeric_type len)
+  val one = wordsSyntax.mk_wordii(1, len)
+  
+  val premise = mk_neg(mk_eq(fixwidth_n, fixwidth_0))
+  val sub1 = wordsSyntax.mk_word_sub(v2w_n, one)
+  val lhs = wordsSyntax.mk_word_ls(v2w_l, sub1)
+  val rhs = mk_neg(wordsSyntax.mk_word_hs(v2w_l, v2w_n))
+  val conclusion = mk_eq(lhs, rhs)
+  val goal = list_mk_forall([n_var, lval_var], mk_imp(premise, conclusion))
+
+  val thm = prove(goal,
+                  rpt strip_tac >>
+                  Cases_on `^v2w_n = v2w (n2v 0)` >-
+                   gvs[v2w_11] >> gvs[] >> 
+                  imp_res_tac word_ineq_all1_thm >>
+                  gvs[]
+                 )
+in
+  thm
+end;
+
+                    
+val word_ineq2_thms = List.tabulate(128, fn i => prove_ineq2_thm (i+1));
+val word_ineq_all2 = LIST_CONJ word_ineq2_thms;
+val word_ineq_all2_thm = save_thm("word_ineq_all_sizes2", word_ineq_all2);
+
+
+    
+
+Theorem bitv_binpred_ge_bool_conv1:
+  ∀ lval_bl n n' len bool.
+    fixwidth len n ≠ fixwidth len (n2v 0) ∧
+    len > 0 ∧ len < 129 ∧
+    bitv_binop binop_sub (n,len) (n2v 1,len) = SOME n' ∧
+    bitv_binpred binop_ge (lval_bl,len) (n,len) = SOME bool ⇒
+    bitv_binpred binop_le (lval_bl,len) n' = SOME (¬bool)
+Proof             
+                                                
+  rpt strip_tac >>
+  PairCases_on ‘n'’ >>
+  imp_res_tac bitv_binop_range_length >>
+  gvs[] >>
+  
+  gvs[bitv_binpred_def, bitv_binop_def] >>                                                      
+  RW.ONCE_RW_TAC [bitv_binpred_inner_def, bitv_binop_inner_def] >>
+  rpt strip_tac >>
+  
+rpt (    
+  BasicProvers.FULL_CASE_TAC >-
+   (
+   fs[] >>
+   gvs[bitv_binop_inner_def, bitv_binpred_inner_def] >>
+   gvs[get_word_binpred_def, get_word_binop_def] >>
+   fs[] >>
+   
+   rewrite_tac [Once $ GSYM word_sub_def] >>
+   
+   imp_res_tac word_ineq_all2_thm >>
+   gvs[]
+   )
+  ) >>
+  intLib.COOPER_TAC
+QED
+
+                                                
+
+
+
+        
+Theorem bs_op_means_same_length:
+  ∀ op lval_bs v_bs x.        
+    SOME x = bitv_binpred op lval_bs v_bs ⇒
+    (SND lval_bs = SND v_bs)
+Proof
+  rpt strip_tac >>
+  PairCases_on ‘lval_bs’ >>
+  PairCases_on ‘v_bs’ >>
+  gvs[bitv_binpred_def]
+QED
+     
+
+
+Theorem last_edge_of_binpred_bs:
+  ∀ binpred v v' n.
+    n ≠ 0 ∧
+    bitv_binpred_inner binpred v v' n = NONE ⇒
+    n > 128
+Proof
+
+  RW.ONCE_RW_TAC [bitv_binpred_inner_def] >>
+  rpt strip_tac >>
+  ntac 128 (BasicProvers.FULL_CASE_TAC >-
+             fs[]) >>
+  intLib.COOPER_TAC
+QED
+
+
+
+
+Theorem last_edge_of_binop_bs:
+  ∀ binpred v v' n.
+    n ≠ 0 ∧
+    bitv_binop_inner binpred v v' n = NONE ⇒
+    n > 128
+Proof
+
+  RW.ONCE_RW_TAC [bitv_binop_inner_def] >>
+  rpt strip_tac >>
+  ntac 128 (BasicProvers.FULL_CASE_TAC >-
+             fs[]) >>
+  intLib.COOPER_TAC
+QED
+
+
+
+ 
+Theorem no_bs_is_larger_than_the_largest:
+  ∀ n n'.
+    n' ≠ 0 ∧ n' ≤ 128 ⇒
+    bitv_binpred_inner binop_gt n (n2v (max_from_type n')) (n':num) = SOME F
+Proof
+  rw[max_from_type_def] >>
+  RW.ONCE_RW_TAC [bitv_binpred_inner_def] >>
+  rpt strip_tac >>
+  
+  rpt(
+    BasicProvers.FULL_CASE_TAC >-
+     (EVAL_TAC >>
+      intLib.COOPER_TAC)) >>
+  intLib.COOPER_TAC
+QED
+
+
+
+Theorem no_bs_is_less_that_the_least:
+  ∀ n n'.
+    n' ≠ 0 ∧ n' ≤ 128 ⇒
+    bitv_binpred_inner binop_lt n (n2v 0) n' = SOME F
+Proof
+  
+  rw[max_from_type_def] >>
+  RW.ONCE_RW_TAC [bitv_binpred_inner_def] >>
+  rpt strip_tac >>
+  
+  rpt(
+    BasicProvers.FULL_CASE_TAC >- 
+     (EVAL_TAC >>
+      intLib.COOPER_TAC)) >>
+  intLib.COOPER_TAC
+QED
+
+
+
+Theorem max_ge_max_thm:
+  ∀ len.
+    len > 0 ∧ len < 129 ⇒                                                                            
+    bitv_binpred binop_ge (n2v (max_from_type len),len) (n2v (max_from_type len),len) = SOME T
+Proof
+
+  rw[max_from_type_def] >>
+  RW.ONCE_RW_TAC [bitv_binpred_def] >>
+  gvs[] >>
+  rpt strip_tac >>
+  RW.ONCE_RW_TAC [bitv_binpred_inner_def] >>
+  
+  rewrite_tac[get_word_binpred_def] >>
+  
+                 
+  rpt(
+    BasicProvers.FULL_CASE_TAC >-
+     fs[] 
+    ) >>
+  intLib.ARITH_TAC
+QED
+
+
+
+
+
+
+
+Theorem every_bs_is_less_than_max:
+  ∀ bl len.
+    len > 0 ∧ len < 129 ⇒
+    bitv_binpred binop_le (bl,len) (n2v (max_from_type len),len) = SOME T
+Proof
+  rw[max_from_type_def] >>
+  RW.ONCE_RW_TAC [bitv_binpred_def] >>
+  gvs[] >>
+  rpt strip_tac >>
+  RW.ONCE_RW_TAC [bitv_binpred_inner_def] >>
+  
+  rewrite_tac[get_word_binpred_def] >>
+  
+  
+  rpt(
+    BasicProvers.FULL_CASE_TAC >-
+     (fs[] >>
+      blastLib.FULL_BBLAST_TAC) 
+    ) >>
+  
+  intLib.ARITH_TAC
+QED                
+
+
+
+(*
+(∀a b. a <₊ n2w (max_from_type n) ⇒ (a + 1w ≤₊ b ⇔ a <₊ b))
+*)
+
+        
+fun gen_max_bound_thm len =
+let
+  val size_term = numSyntax.term_of_int len
+  val word_ty = wordsSyntax.mk_int_word_type len
+                            
+    val a = mk_var("a", word_ty)
+    val b = mk_var("b", word_ty)
+  
+  val goal = 
+    ``∀ a b. ^a <₊ n2w (max_from_type ^size_term) ⇒ 
+      (^a + 1w ≤₊ ^b ⇔ ^a <₊ ^b)``;
+  
+  val thm = prove(goal,
+                 gvs[max_from_type_def] >>
+                 rpt strip_tac >>
+                 blastLib.FULL_BBLAST_TAC )
+in
+  thm
+end;
+
+val gen_max_bound_thms = List.tabulate(128, fn i => gen_max_bound_thm (i+1));
+val gen_max_bound_all1 = LIST_CONJ gen_max_bound_thms;
+val gen_max_bound_all1_thm = save_thm("gen_max_bound_all1_sizes", gen_max_bound_all1);
+
+    
+Theorem bitv_binpred_le_bool_conv1:
+  ∀ len lval_bs n n' bool.
+    len > 0 ∧ len < 129 ∧
+    bitv_binpred binop_le (lval_bs,len) (n,len) = SOME bool ∧
+    bitv_binpred binop_ge (n,len) (n2v (max_from_type len),len) = SOME F ∧
+    bitv_binop binop_add (n,len) (n2v 1,len) = SOME n' ⇒
+    bitv_binpred binop_ge (lval_bs,len) n' = SOME (¬bool)                    
+Proof
+  rpt strip_tac >>
+  PairCases_on ‘n'’ >>
+  imp_res_tac bitv_binop_range_length >>
+  gvs[] >>
+  
+  gvs[bitv_binpred_def, bitv_binop_def] >>                                                      
+  RW.ONCE_RW_TAC [bitv_binpred_inner_def, bitv_binop_inner_def] >>
+  rpt strip_tac >>
+  
+  rpt(
+    BasicProvers.FULL_CASE_TAC >-
+     (
+     fs[] >>
+     gvs[bitv_binop_inner_def, bitv_binpred_inner_def] >>
+     gvs[get_word_binpred_def, get_word_binop_def] >>
+     fs[] >>
+     
+     
+     
+     rpt strip_tac >>
+     gvs[WORD_HIGHER_EQ] >>
+     gvs[WORD_NOT_LOWER_EQUAL] >>
+     gvs[gen_max_bound_all1_thm]
+     )
+    ) >> intLib.ARITH_TAC
+QED 
+    
+
+
+
+
+val _ = export_theory ();
+
+    
+
